LinearScan/seq.hs
@@ -1,6 +1,3 @@
-{-# OPTIONS_GHC -cpp -fglasgow-exts #-}
-{- For Hugs, use the option -F"cpp -P -traditional" -}
-
 module LinearScan.Seq where
 
 import qualified Prelude
@@ -10,42 +7,11 @@ import qualified LinearScan.Eqtype as Eqtype
 import qualified LinearScan.Ssrbool as Ssrbool
 
 
-
---unsafeCoerce :: a -> b
-#ifdef __GLASGOW_HASKELL__
-import qualified GHC.Base as GHC.Base
-unsafeCoerce = GHC.Base.unsafeCoerce#
-#else
--- HUGS
-import qualified LinearScan.IOExts as IOExts
-unsafeCoerce = IOExts.unsafeCoerce
-#endif
-
 has :: (Ssrbool.Coq_pred a1) -> ([] a1) -> Prelude.Bool
 has a s =
   case s of {
    [] -> Prelude.False;
    (:) x s' -> (Prelude.||) (a x) (has a s')}
-
-mem_seq :: Eqtype.Equality__Coq_type -> ([] Eqtype.Equality__Coq_sort) ->
-           Eqtype.Equality__Coq_sort -> Prelude.Bool
-mem_seq t s =
-  case s of {
-   [] -> (\x -> Prelude.False);
-   (:) y s' ->
-    let {p = mem_seq t s'} in (\x -> (Prelude.||) (Eqtype.eq_op t x y) (p x))}
-
-type Coq_eqseq_class = [] Eqtype.Equality__Coq_sort
-
-pred_of_eq_seq :: Eqtype.Equality__Coq_type -> Coq_eqseq_class ->
-                  Ssrbool.Coq_pred_sort Eqtype.Equality__Coq_sort
-pred_of_eq_seq t s =
-  unsafeCoerce (\x -> mem_seq t s x)
-
-seq_predType :: Eqtype.Equality__Coq_type -> Ssrbool.Coq_predType
-                Eqtype.Equality__Coq_sort
-seq_predType t =
-  Ssrbool.mkPredType (unsafeCoerce (pred_of_eq_seq t))
 
 rem :: Eqtype.Equality__Coq_type -> Eqtype.Equality__Coq_sort -> ([]
        Eqtype.Equality__Coq_sort) -> [] Eqtype.Equality__Coq_sort
