LinearScan/ssrbool.hs
@@ -1,22 +1,10 @@
-{-# OPTIONS_GHC -cpp -fglasgow-exts #-}
-{- For Hugs, use the option -F"cpp -P -traditional" -}
-
 module LinearScan.Ssrbool where
 
 import qualified Prelude
 import qualified Data.List
 import qualified LinearScan.Utils
+import qualified LinearScan.Ssrfun as Ssrfun
 
-
---unsafeCoerce :: a -> b
-#ifdef __GLASGOW_HASKELL__
-import qualified GHC.Base as GHC.Base
-unsafeCoerce = GHC.Base.unsafeCoerce#
-#else
--- HUGS
-import qualified LinearScan.IOExts as IOExts
-unsafeCoerce = IOExts.unsafeCoerce
-#endif
 
 __ :: any
 __ = Prelude.error "Logical or arity value used"
@@ -39,33 +27,26 @@ idP b1 =
    Prelude.True -> ReflectT;
    Prelude.False -> ReflectF}
 
+andP :: Prelude.Bool -> Prelude.Bool -> Coq_reflect
+andP b1 b2 =
+  case b1 of {
+   Prelude.True ->
+    case b2 of {
+     Prelude.True -> ReflectT;
+     Prelude.False -> ReflectF};
+   Prelude.False -> ReflectF}
+
 type Coq_pred t = t -> Prelude.Bool
 
 type Coq_rel t = t -> Coq_pred t
 
-data Coq_mem_pred t =
-   Mem (Coq_pred t)
+type Coq_simpl_rel t = Ssrfun.Coq_simpl_fun t (Coq_pred t)
 
-data Coq_predType t =
-   PredType (() -> Coq_pred t) (() -> Coq_mem_pred t)
+coq_SimplRel :: (Coq_rel a1) -> Coq_simpl_rel a1
+coq_SimplRel r =
+  Ssrfun.SimplFun (\x -> r x)
 
-type Coq_pred_sort t = ()
-
-mkPredType :: (a2 -> a1 -> Prelude.Bool) -> Coq_predType a1
-mkPredType toP =
-  PredType (unsafeCoerce toP) (\p -> Mem (\x -> unsafeCoerce toP p x))
-
-pred_of_mem :: (Coq_mem_pred a1) -> Coq_pred_sort a1
-pred_of_mem mp =
-  case mp of {
-   Mem p -> unsafeCoerce (\x -> p x)}
-
-mem :: (Coq_predType a1) -> (Coq_pred_sort a1) -> Coq_mem_pred a1
-mem pT =
-  case pT of {
-   PredType topred s -> s}
-
-in_mem :: a1 -> (Coq_mem_pred a1) -> Prelude.Bool
-in_mem x mp =
-  unsafeCoerce (\_ -> pred_of_mem) __ mp x
+rel_of_simpl_rel :: (Coq_simpl_rel a1) -> Coq_rel a1
+rel_of_simpl_rel r x y =
+  Ssrfun.fun_of_simpl r x y
 
