LinearScan/ssrfun.hs
@@ -1,0 +1,14 @@
+module LinearScan.Ssrfun where
+
+import qualified Prelude
+import qualified Data.List
+import qualified LinearScan.Utils
+
+data Coq_simpl_fun aT rT =
+   SimplFun (aT -> rT)
+
+fun_of_simpl :: (Coq_simpl_fun a1 a2) -> a1 -> a2
+fun_of_simpl f x =
+  case f of {
+   SimplFun lam -> lam x}
+
