Spec.v
@@ -1,0 +1,537 @@
+Require Import Lib.
+
+Require Export Machine.
+Require Export Interval.
+Require Export ScanState.
+
+Set Implicit Arguments.
+Unset Strict Implicit.
+Unset Printing Implicit Defensive.
+Generalizable All Variables.
+
+Module MLinearSpec (Mach : Machine).
+Import Mach.
+Module Import MS := MScanState Mach.
+
+Import EqNotations.
+
+Definition maxReg := maxReg.
+Definition PhysReg := fin maxReg.
+Definition registers_exist := registers_exist.
+
+(** * Linear scan specification *)
+
+(** This module contains Theorems which prove properties concerning the
+    specification the linear register allocation algorithm, but which are not
+    directly used in implementing the algorithm. *)
+
+Lemma Forall_widen : forall n x (xs : list (fin n * nat)),
+  List.Forall (lebf snd x) xs
+    -> List.Forall (lebf snd (widen_id (fst x), snd x))
+                   [seq (widen_id (fst p), snd p) | p <- xs].
+Proof.
+  move=> ? x xs.
+  elim: xs x => //= [? ? IHys] ? H /=.
+  constructor; first by inv H.
+  by apply IHys; inv H.
+Qed.
+
+Lemma StronglySorted_widen : forall n (xs : list (fin n * nat)),
+  StronglySorted (lebf snd) xs
+    -> StronglySorted (lebf snd) [seq (widen_id (fst p), snd p) | p <- xs].
+Proof.
+  move=> ?.
+  elim=> /= [|? ? ?] H; first by constructor.
+  constructor; first by inv H.
+  by apply Forall_widen; inv H.
+Qed.
+
+Theorem unhandled_sorted `(st : ScanState sd) :
+  StronglySorted (lebf snd) (unhandled sd).
+Proof.
+  ScanState_cases (induction st) Case.
+  - Case "ScanState_nil". constructor.
+
+  - Case "ScanState_newUnhandled".
+    rewrite /unh.
+    by apply/StronglySorted_insert_spec/StronglySorted_widen/IHst.
+
+  - Case "ScanState_moveUnhandledToActive". inv IHst.
+  - Case "ScanState_moveActiveToInactive". apply IHst.
+  - Case "ScanState_moveActiveToHandled". apply IHst.
+  - Case "ScanState_moveInactiveToActive". apply IHst.
+  - Case "ScanState_moveInactiveToHandled".  apply IHst.
+
+  - Case "ScanState_splitCurrentInterval".
+    rewrite /unhandled /unh' in IHst *.
+    apply StronglySorted_insert_spec.
+    apply StronglySorted_inv in IHst.
+    move: IHst => [H1 H2].
+    apply: StronglySorted_widen.
+    by constructor.
+Qed.
+
+Lemma uniq_rem : forall n x (xs : seq (fin n * PhysReg)),
+  uniq [seq snd i | i <- xs] -> uniq [seq snd i | i <- rem x xs].
+Proof.
+  move=> n x.
+  elim=> [|y ys IHys] Huniq //=.
+  move: cons_uniq Huniq => -> /andP [H1 H2].
+  case: (y == x); first by [].
+  rewrite cons_uniq.
+  apply/andP; split.
+    admit.
+  by apply IHys.
+Qed.
+
+Lemma in_snd_trans : forall (a b : eqType) (x : a * b) (xs ys : seq (a * b)),
+  x \in xs -> ~~ has (mem [seq snd i | i <- xs]) [seq snd i | i <- ys]
+    -> snd x \notin [seq snd i | i <- ys].
+Admitted.
+
+Theorem active_regs_are_unique `(st : ScanState sd) :
+  uniq ([ seq snd i | i <- active sd ] ++ [ seq snd i | i <- inactive sd ]).
+Proof.
+  ScanState_cases (induction st) Case.
+  - Case "ScanState_nil". constructor.
+  - Case "ScanState_newUnhandled".
+    by rewrite /widen_fst -!map_comp /funcomp //.
+  - Case "ScanState_moveUnhandledToActive".
+    move: map_cat => /= <- in IHst *; apply/andP.
+    admit.
+
+  - Case "ScanState_moveActiveToInactive".
+    move: IHst.
+    rewrite /= !cat_uniq.
+    move/and3P=> [H1 H2 H3].
+    apply/and3P; split.
+    + by apply/uniq_rem.
+    + admit.
+    + rewrite cons_uniq.
+      apply/andP; split; last by [].
+      by apply in_snd_trans with (xs := active sd).
+
+  - Case "ScanState_moveActiveToHandled".
+    move: IHst.
+    rewrite /= !cat_uniq.
+    move/and3P=> [H1 H2 H3].
+    apply/and3P; split; last by [].
+      by apply/uniq_rem.
+    admit.
+
+  - Case "ScanState_moveInactiveToActive".
+    simpl in *.
+    apply/andP; split.
+      admit.
+    admit.
+
+  - Case "ScanState_moveInactiveToHandled".
+    move: IHst.
+    rewrite /= !cat_uniq.
+    move/and3P=> [H1 H2 H3].
+    apply/and3P; split; first by [].
+      admit.
+    by apply/uniq_rem.
+
+  - Case "ScanState_splitCurrentInterval".
+    by rewrite /widen_fst -!map_comp /funcomp //.
+Qed.
+
+(** The number of active or inactive registers cannot exceed the number of
+    registers available (or, if there are more register than intervals to be
+    allocated, the number of intervals). *)
+Theorem limit_active_registers `(st : ScanState sd) :
+  size (active sd ++ inactive sd) <= minn maxReg (nextInterval sd).
+Admitted.
+
+Lemma move_unhandled_to_active : forall n (x : fin n) unh act inact hnd,
+  uniq ((x :: unh) ++ act ++ inact ++ hnd)
+    -> uniq (unh ++ (x :: act) ++ inact ++ hnd).
+Proof. by intros; rewrite cat_cons -cat1s uniq_catCA cat1s -cat_cons. Qed.
+
+Lemma uniq_juggle : forall n (a : eqType) (xs ys : list (fin n * a)) zs,
+  uniq ([seq fst i | i <- xs] ++ [seq fst i | i <- ys] ++ zs)
+    -> forall x, x \in xs
+    -> uniq ([seq fst i | i <- rem x xs] ++ [seq fst i | i <- x :: ys] ++ zs).
+Proof.
+  move=> n a.
+  elim=> [|x xs IHxs] ys zs H x0 Hin //=.
+  case E: (x == x0) => /=.
+    move: E => /eqP <-.
+    by rewrite -cat1s uniq_catCA cat1s -cat_cons.
+  apply/andP.
+  split.
+    rewrite !mem_cat.
+    move: cat_uniq H => -> /and3P => [[H1 H2 H3]].
+    move: cons_uniq H1 => -> /andP => [[H4 H5]].
+    rewrite negb_orb.
+    apply/andP.
+    apply negbT in E.
+    split. admit. (* exact: not_in_rem. *)
+    rewrite has_sym in H2.
+    inversion H2 as [H2'].
+    move: negb_orb H2' => -> /andP [H6 H7].
+    rewrite in_cons negb_orb.
+    apply/andP. split. admit. admit.
+  apply IHxs.
+    inversion H as [H'].
+    by move: H' => /andP [_ ?].
+  move: in_cons Hin => -> /orP [He|_] //.
+  move: eq_sym E He => -> /eqP E /eqP He.
+  contradiction.
+Qed.
+
+Lemma move_active_to_inactive : forall sd x,
+  uniq (unhandledIds sd ++ activeIds sd ++ inactiveIds sd ++ handledIds sd)
+    -> x \in active sd
+    -> uniq (unhandledIds sd ++ [seq fst i | i <- rem x (active sd)] ++
+              [seq fst i | i <- x :: inactive sd] ++ handledIds sd).
+Proof.
+  intros.
+  rewrite uniq_catC -catA -catA.
+  apply uniq_juggle.
+    by rewrite catA catA uniq_catC -catA.
+  exact: H0.
+Qed.
+
+Lemma move_active_to_handled : forall sd x,
+  uniq (unhandledIds sd ++ activeIds sd ++ inactiveIds sd ++ handledIds sd)
+    -> x \in active sd
+    -> uniq (unhandledIds sd ++ [seq fst i | i <- rem x (active sd)] ++
+              inactiveIds sd ++ [seq fst i | i <- x :: handled sd]).
+Proof.
+  intros.
+  rewrite uniq_catC -catA -catA uniq_catCA2 -catA.
+  apply uniq_juggle.
+    by rewrite catA uniq_catCA2 catA uniq_catC -catA catA uniq_catCA2 -catA.
+  exact: H0.
+Qed.
+
+Lemma move_inactive_to_active : forall sd x,
+  uniq (unhandledIds sd ++ activeIds sd ++ inactiveIds sd ++ handledIds sd)
+    -> x \in inactive sd
+    -> uniq (unhandledIds sd ++ [seq fst i | i <- x :: active sd] ++
+              [seq fst i | i <- rem x (inactive sd)] ++ handledIds sd).
+Proof.
+  intros.
+Admitted.
+(*   rewrite -cat_cons uniq_catC -catA uniq_catC -!catA *)
+(*           (catA (handled sd)) uniq_catCA2. *)
+(*   apply uniq_juggle. *)
+(*     by rewrite !catA uniq_catC -catA uniq_catCA2 -catA catA uniq_catCA2 -catA. *)
+(*   exact: H0. *)
+(* Qed. *)
+
+Lemma move_inactive_to_handled : forall sd x,
+  uniq (unhandledIds sd ++ activeIds sd ++ inactiveIds sd ++ handledIds sd)
+    -> x \in inactive sd
+    -> uniq (unhandledIds sd ++ activeIds sd
+               ++ [seq fst i | i <- rem x (inactive sd)]
+               ++ [seq fst i | i <- x :: handled sd]).
+Proof.
+  intros.
+  rewrite (catA (unhandledIds sd)) uniq_catC -!catA.
+  apply uniq_juggle.
+    admit.
+    (* by rewrite (catA (inactive sd)) uniq_catC -!catA. *)
+  exact: H0.
+Qed.
+
+Lemma notin_fst : forall n P x y (xs : seq (fin n * nat)),
+  fst x != fst y
+    -> @fst _ nat y \notin [seq fst i | i <- xs]
+    -> fst y \notin [seq fst i | i <- insert (P ^~ x) x xs].
+Proof.
+  move=> n P x y.
+  elim=> /= [|z zs IHzs] Heqe H.
+    by rewrite mem_seq1 eq_sym.
+  move: H.
+  rewrite in_cons negb_orb => /andP [H1 H2].
+  rewrite /insert.
+  case E: (P z x).
+    rewrite map_cons in_cons negb_orb.
+    apply/andP; split. by [].
+    exact: IHzs.
+  rewrite map_cons in_cons negb_orb.
+  apply/andP; split.
+    by rewrite eq_sym.
+  rewrite map_cons in_cons negb_orb.
+  by apply/andP.
+Qed.
+
+Lemma uniq_insert_cons :
+  forall n P (f : fin n -> fin (S n)) x (xs : seq (fin n * nat)),
+  uniq [seq fst i | i <- x :: xs]
+    -> uniq [seq fst i | i <- insert (P ^~ x) x xs].
+Proof.
+  move=> n P f x.
+  elim=> //= y ys IHys /and3P [H1 ? ?].
+  move: H1.
+  rewrite in_cons negb_orb => /andP [? ?].
+  rewrite /insert.
+  case E: (P y x).
+    rewrite map_cons cons_uniq.
+    apply/andP; split.
+      exact: notin_fst.
+    by apply/IHys/andP.
+  rewrite !map_cons !cons_uniq.
+  rewrite in_cons negb_orb.
+  apply/and3P; split; auto.
+  by apply/andP.
+Qed.
+
+Lemma map_f_notin :
+  forall (T1 T2 : eqType) (f : T1 -> T2) (s : seq T1) (x : T1),
+  injective f -> x \notin s -> f x \notin [seq f i | i <- s].
+Proof.
+  move=> T1 T2 f.
+  elim=> // x xs IHxs x0 Hinj.
+  rewrite in_cons negb_orb => /andP [H1 H2].
+  rewrite map_cons in_cons negb_orb.
+  apply/andP; split.
+    by rewrite inj_eq.
+  exact: IHxs.
+Qed.
+
+Lemma uniq_trans_fst :
+  forall n (f : fin n -> fin (S n)) (xs : seq (fin n * nat)),
+  injective f
+    -> uniq [seq fst i | i <- xs]
+    -> uniq [seq fst i | i <- [seq (fun p => (f (fst p), snd p)) p | p <- xs]].
+Proof.
+  move=> n f.
+  elim=> // x xs IHxs Hinj.
+  rewrite map_cons cons_uniq => /andP [H1 H2].
+  rewrite -map_comp map_cons map_comp /=.
+  apply/andP; split.
+    rewrite -map_comp.
+    replace ([eta fst] \o (fun p : fin n * nat => (f (fst p), snd p)))
+       with (f \o @fst _ nat); last by [].
+    rewrite map_comp.
+    exact: map_f_notin.
+  exact: IHxs.
+Qed.
+
+Lemma no_ord_max : forall n (xs : seq (fin n * nat)),
+   ord_max \notin [ seq fst i | i <- [seq widen_fst p | p <- xs] ].
+Proof.
+  move=> n.
+  elim=> // x xs IHxs.
+  rewrite -map_comp map_cons in_cons negb_orb /=.
+  apply/andP; split.
+    apply lift_bounded.
+  rewrite map_comp.
+  apply IHxs.
+Qed.
+
+Lemma in_map_inj : forall n x xs,
+  let f := widen_ord (leqnSn n) in
+  x \in [seq f i | i <- xs] -> { y | x = f y & y \in xs }.
+Proof.
+  move=> n x xs.
+  elim E: xs => //= [y ys IHys] Hin.
+  case X: (x == widen_ord (leqnSn n) y).
+    exists y. by apply/eqP/X.
+    rewrite in_cons.
+    by apply/orP; left.
+  move: map_cons in_cons X Hin => -> -> ->.
+  rewrite orb_false_l => Hin.
+  specialize (IHys Hin).
+  case: IHys => z Heqe2 Hin2.
+  exists z. by [].
+  case Y: (y == z).
+    rewrite in_cons eq_sym.
+    by apply/orP; left.
+  rewrite in_cons.
+  by apply/orP; right.
+Defined.
+
+Lemma not_in_widen : forall n (xs : seq (fin n * nat)) z,
+  let f := widen_ord (leqnSn n) in
+  z \notin [seq fst i | i <- xs]
+    -> f z \notin [seq fst i | i <- [seq (f (fst p), snd p) | p <- xs]].
+Proof.
+  move=> n.
+  elim=> //= x xs IHxs z Hni.
+  move: Hni.
+  rewrite in_cons negb_orb => /andP [H1 H2].
+  rewrite in_cons negb_orb.
+  apply/andP; split. by [].
+  exact: IHxs.
+Qed.
+
+Lemma not_mem_insert_cons :
+  forall n (x : fin n.+1 * nat) (xs : seq (fin n * nat)) z,
+  let f := widen_ord (leqnSn n) in
+  let xs' : seq (fin n.+1 * nat) := [seq (f (fst p), snd p) | p <- xs] in
+  fst x != f z
+    -> ~~ (mem [seq fst i | i <- xs]) z
+    -> ~~ (mem [seq fst i | i <- insert ((lebf snd)^~ x) x
+                  [seq (f (fst p), snd p) | p <- xs]]) (f z).
+Proof.
+  move=> n x.
+  elim=> //= [|y ys IHys] z Hne Hmem.
+    by rewrite mem_seq1 eq_sym.
+  move: Hmem. rewrite in_cons negb_orb => /andP [? ?].
+  rewrite /insert.
+  case E: (lebf snd (widen_ord (leqnSn n) (fst y), snd y) x).
+    rewrite map_cons in_cons negb_orb.
+    apply/andP; split. by [].
+    exact: IHys.
+  rewrite map_cons in_cons negb_orb.
+  apply/andP; split.
+    by rewrite eq_sym.
+  rewrite map_cons in_cons negb_orb.
+  apply/andP; split. by [].
+  exact: not_in_widen.
+Qed.
+
+Lemma uniq_1st_of_four (T : eqType) (xs1 xs2 : seq T) : forall (ys : seq T),
+  uniq xs1 == uniq xs2 -> uniq (xs1 ++ ys) == uniq (xs2 ++ ys).
+Admitted.
+
+Lemma unhandled_insert_uniq : forall n beg xs ys,
+  let wf := @widen_fst n _ in
+  let x  := (ord_max, beg) in
+  uniq ([seq fst i | i <- xs] ++ ys)
+    -> uniq ([seq fst i | i <- insert (lebf snd ^~ x) x (map wf xs)] ++
+             map widen_id ys).
+Proof.
+  move=> n beg xs ys wf x IHst.
+Admitted.
+(*   rewrite -!map_cat cat_uniq => /=. *)
+(*   move: IHst. *)
+(*   rewrite cat_uniq => /and3P [H2 H3 H4]. *)
+(*   apply/and3P; split. *)
+(*   + apply uniq_insert_cons. *)
+(*       exact: widen_ord. *)
+(*     rewrite map_cons /=. *)
+(*     apply/andP; split. *)
+(*       exact: no_ord_max. *)
+(*     apply uniq_trans_fst. *)
+(*       exact: widen_ord_inj. *)
+(*     by []. *)
+(*   + move: H3 => /hasPn H3. *)
+(*     apply/hasPn. move=> ? Hin. *)
+(*     apply in_map_inj in Hin. *)
+(*     set f := widen_ord (leqnSn n). *)
+(*     case: Hin => y -> Hin. *)
+(*     have Hne: fst x != f y. *)
+(*       by apply lift_bounded. *)
+(*     by apply/not_mem_insert_cons/(H3 y Hin). *)
+(*   + rewrite map_inj_uniq. by []. *)
+(*     exact: widen_ord_inj. *)
+(* Qed. *)
+
+Theorem lists_are_unique `(st : ScanState sd) : uniq (all_state_lists sd).
+Proof.
+  rewrite /all_state_lists /unhandledIds /IntervalId.
+  ScanState_cases (induction st) Case.
+  - Case "ScanState_nil". by [].
+  - Case "ScanState_newUnhandled".
+    rewrite /unhandledIds /activeIds /inactiveIds /handledIds. simpl.
+    move: cat_uniq IHst => -> /and3P [H1 H2 H3].
+    rewrite cat_uniq.
+    apply/and3P; split.
+    + admit.
+    + admit.
+    + admit.
+  - Case "ScanState_moveUnhandledToActive".
+    exact: move_unhandled_to_active.
+  - Case "ScanState_moveActiveToInactive".
+    exact: (@move_active_to_inactive _ x IHst H).
+  - Case "ScanState_moveActiveToHandled".
+    exact: (@move_active_to_handled _ x IHst H).
+  - Case "ScanState_moveInactiveToActive".
+    exact: (@move_inactive_to_active _ x IHst H).
+  - Case "ScanState_moveInactiveToHandled".
+    exact: (@move_inactive_to_handled _ x IHst H).
+  - Case "ScanState_splitCurrentInterval".
+    (* exact: unhandled_insert_uniq. *)
+    admit.
+Qed.
+
+Theorem all_intervals_represented `(st : ScanState sd) :
+  size (all_state_lists sd) == nextInterval sd.
+Proof.
+  rewrite /all_state_lists /unhandledIds /IntervalId /nextInterval.
+  ScanState_cases (induction st) Case.
+  - Case "ScanState_nil". by [].
+
+  - Case "ScanState_newUnhandled".
+    rewrite !size_cat !size_map ?size_insert /=.
+    by move: IHst; rewrite !size_cat !size_map /=.
+
+  - Case "ScanState_moveUnhandledToActive".
+    rewrite !size_cat size_map /=.
+    by move: IHst; rewrite !size_cat size_map /= addnS.
+
+  - Case "ScanState_moveActiveToInactive".
+    admit.
+    (* rewrite !size_cat size_map size_rem /=; last by []. *)
+    (* move: IHst; rewrite !size_cat size_map /=. *)
+    (* case E: (active sd). by rewrite E in H; inv H. *)
+    (* by rewrite [_.-1 + _]addnC addSn -[_ + _.-1]addnC -addSn /=. *)
+
+  - Case "ScanState_moveActiveToHandled".
+    admit.
+    (* rewrite !size_cat size_map size_rem /=; last by []. *)
+    (* move: IHst; rewrite !size_cat size_map. *)
+    (* case E: (active sd). by rewrite E in H; inv H. *)
+    (* by rewrite 2!addnS -addSn /=. *)
+
+  - Case "ScanState_moveInactiveToActive".
+    admit.
+    (* rewrite -cat_cons !size_cat size_map size_rem /=; last by []. *)
+    (* move: IHst; rewrite !size_cat size_map /=. *)
+    (* case E: (inactive sd). rewrite E in H. inv H. *)
+    (* by rewrite 2!addnS -addSn /=. *)
+
+  - Case "ScanState_moveInactiveToHandled".
+    admit.
+    (* rewrite !size_cat size_map size_rem /=; last by []. *)
+    (* move: IHst; rewrite !size_cat size_map /=. *)
+    (* case E: (inactive sd). rewrite E in H. inv H. *)
+    (* by rewrite 2!addnS -addSn /=. *)
+
+  - Case "ScanState_splitCurrentInterval".
+    rewrite /unhandled /active /inactive /handled in IHst *.
+    rewrite !size_cat !size_map size_insert /=.
+    by move: IHst; rewrite !size_cat !size_map /=.
+Qed.
+
+(* jww (2014-10-25): Proving this will require that the constructor accepts a
+   proof that there is romo in the active pool, and then in tryAllocateFreeReg
+   is when we split based on whether that list is full or not (for this is
+   what causes allocation there to fail).  With the knowledge of that split,
+   we would then know that there is either room, or no room (but after
+   spilling there should then be room again).
+
+   But rather than taking the size of the active list to determine this, we
+   would have another lemma stating that if the algorithm that determines
+   freeUntilPos fails to find a free register, this implies that size (active
+   sd) == maxReg. *)
+(*
+Theorem actives_within_range `(st : ScanState sd) :
+  size (active sd) <= maxReg.
+Proof.
+  ScanState_cases (induction st) Case; simpl in *.
+  - Case "ScanState_nil". by [].
+  - Case "ScanState_newUnhandled".
+    by rewrite size_map.
+  - Case "ScanState_moveUnhandledToActive". (* TODO *)
+  - Case "ScanState_moveActiveToInactive".
+    rewrite size_rem; last by [].
+    case E: (active sd) => //=.
+    by rewrite E /= in IHst; apply ltnW.
+  - Case "ScanState_moveActiveToHandled".
+    rewrite size_rem; last by [].
+    case E: (active sd) => //=.
+    by rewrite E /= in IHst; apply ltnW.
+  - Case "ScanState_moveInactiveToActive". (* TODO *)
+  - Case "ScanState_moveInactiveToHandled".
+    by [].
+Qed.
+*)
+
+End MLinearSpec.
